Sem.v
@@ -8,24 +8,23 @@ From Elo Require Import Map.
 
 Definition id   := string.
 Definition addr := nat.
-Definition lock := nat.
  
 (* ------------------------------------------------------------------------- *)
 (* types                                                                     *)
 (* ------------------------------------------------------------------------- *)
 
 (* safe type *)
-Inductive styp : Set :=
+Inductive sty : Set :=
   | ty_unit
   | ty_num
-  | ty_refS : styp -> styp
-  | ty_mtx  : typ -> styp
+  | ty_refR : sty -> sty (* read reference *)
+  | ty_refX : ty  -> sty (* guarded reference *)
 
 (* type *)
-with typ : Set :=
-  | ty_safe : styp -> typ
-  | ty_refU : typ  -> typ
-  | ty_fun  : typ  -> typ -> typ
+with ty : Set :=
+  | ty_safe : sty -> ty
+  | ty_refW : ty  -> ty (* write reference *)
+  | ty_fun  : ty  -> ty -> ty
   .
 
 (* ------------------------------------------------------------------------- *)
@@ -38,106 +37,94 @@ Inductive tm : Set :=
   | tm_nat   : nat -> tm
   (* functions *)
   | tm_var   : id -> tm
-  | tm_fun   : id -> typ -> tm -> tm
-  | tm_call  : tm -> tm  -> tm
+  | tm_fun   : id -> ty -> tm -> tm
+  | tm_call  : tm -> tm -> tm
   (* memory *)
-  | tm_ref   : addr -> typ -> tm
-  | tm_new   : typ  -> tm  -> tm
+  | tm_ref   : addr -> ty -> tm
+  | tm_new   : tm   -> ty -> tm
   | tm_load  : tm   -> tm
-  | tm_asg   : tm   -> tm  -> tm
+  | tm_asg   : tm   -> tm -> tm
+  | tm_acq   : tm   -> tm -> tm
+  | tm_cr    : addr -> tm -> tm       (* critical region  *)
+  | tm_ptm   : option nat -> tm -> tm (* protected term   *)
   (* concurrency *)
   | tm_spawn : tm -> tm
-  (* mutual exclusion *)
-  | tm_mtx   : lock -> tm -> tm
-  | tm_newx  : tm -> tm
-  | tm_acq   : tm -> tm -> tm
-  | tm_cr    : lock -> tm -> tm
   .
 
 (* ------------------------------------------------------------------------- *)
 (* notations                                                                 *)
 (* ------------------------------------------------------------------------- *)
 
-Declare Custom Entry elo_typ.
-Notation "<{{ T }}>" := T (T custom elo_typ at level 99).
-Notation "( x )"     := x (in custom elo_typ, x at level 99).
-Notation "x"         := x (in custom elo_typ at level 0, x constr at level 0).
+(* types *)
+Declare Custom Entry elo_ty.
+Notation "` T `" := T (T custom elo_ty at level 99).
+Notation "( x )" := x (in custom elo_ty, x at level 99).
+Notation "x"     := x (in custom elo_ty at level 0, x constr at level 0).
 
 (* safe types *)
-Notation "'Unit'"  := (ty_safe ty_unit)          (in custom elo_typ at level 0).
-Notation "'Num'"   := (ty_safe ty_num)           (in custom elo_typ at level 0).
-Notation "'s&' T"  := (ty_safe (ty_refS T))      (in custom elo_typ at level 5).
-Notation "'Mtx' T" := (ty_safe (ty_mtx T))       (in custom elo_typ at level 0).
+Notation "'Unit'" := (ty_safe ty_unit)            (in custom elo_ty at level 0).
+Notation "'Num'"  := (ty_safe ty_num)             (in custom elo_ty at level 0).
+Notation "'r&' T" := (ty_safe (ty_refR T))        (in custom elo_ty at level 5).
+Notation "'x&' T" := (ty_safe (ty_refX T))        (in custom elo_ty at level 5).
 
-(* types *)
-Notation "'Safe' T"    := (ty_safe T)            (in custom elo_typ at level 5).
-Notation "'u&' T"      := (ty_refU T)            (in custom elo_typ at level 5).
-Notation "T1 '-->' T2" := (ty_fun T1 T2)         (in custom elo_typ at level 50,
+(* general types *)
+Notation "'Safe' T"    := (ty_safe T)             (in custom elo_ty at level 5).
+Notation "'w&' T"      := (ty_refW T)             (in custom elo_ty at level 5).
+Notation "T1 '-->' T2" := (ty_fun T1 T2)          (in custom elo_ty at level 50,
                                                            right associativity).
 
+(* terms *)
 Declare Custom Entry elo_tm.
 Notation "<{ t }>" := t (t custom elo_tm at level 99).
-Notation "{ x }"   := x (in custom elo_tm, x at level 99).
+Notation "( x )"   := x (in custom elo_tm, x at level 99).
 Notation "x"       := x (in custom elo_tm at level 0, x constr at level 0).
 
-Notation "'unit'"        := (tm_unit)             (in custom elo_tm at level 0).
-Notation "'nat' n"       := (tm_nat n)            (in custom elo_tm at level 0).
-Notation "'var' x"       := (tm_var x)            (in custom elo_tm at level 0).
-Notation "'fn' x Tx t"   := (tm_fun x Tx t)        (in custom elo_tm at level 0,
+Notation "'unit'"         := (tm_unit)            (in custom elo_tm at level 0).
+Notation "'nat' n"        := (tm_nat n)           (in custom elo_tm at level 0).
+Notation "'var' x"        := (tm_var x)           (in custom elo_tm at level 0).
+Notation "'fn' x Tx t"    := (tm_fun x Tx t)       (in custom elo_tm at level 0,
                                                             x constr at level 0,
-                                                  Tx custom elo_typ at level 0).
-Notation "'call' t1 t2"  := (tm_call t1 t2)       (in custom elo_tm at level 0).
-Notation "'&' ad '::' T" := (tm_ref ad T)          (in custom elo_tm at level 0,
-                                                   T custom elo_typ at level 0).
-Notation "'new' T t"     := (tm_new T t)           (in custom elo_tm at level 0,
-                                                   T custom elo_typ at level 0).
-Notation "'*' t"         := (tm_load t)           (in custom elo_tm at level 0).
-Notation "t1 '=' t2"     := (tm_asg t1 t2)        (in custom elo_tm at level 70,
+                                                   Tx custom elo_ty at level 0).
+Notation "'call' t1 t2"   := (tm_call t1 t2)      (in custom elo_tm at level 0).
+Notation "'&' ad ':' T"   := (tm_ref ad T)         (in custom elo_tm at level 0,
+                                                    T custom elo_ty at level 0).
+Notation "'new' t : T"    := (tm_new t T)          (in custom elo_tm at level 0,
+                                                    T custom elo_ty at level 0).
+Notation "'*' t"          := (tm_load t)          (in custom elo_tm at level 0).
+Notation "t1 ':=' t2"     := (tm_asg t1 t2)       (in custom elo_tm at level 70,
                                                               no associativity).
-Notation "'spawn' t"     := (tm_spawn t)          (in custom elo_tm at level 0).
-Notation "'mtx' l t"     := (tm_mtx l t)          (in custom elo_tm at level 0).
-Notation "'newx' t"      := (tm_newx t)           (in custom elo_tm at level 0).
-Notation "'acq' t1 t2"   := (tm_acq t1 t2)        (in custom elo_tm at level 0).
-Notation "'cr' t1 t2"    := (tm_cr t1 t2)         (in custom elo_tm at level 0).
+Notation "'acq' t1 t2"    := (tm_acq t1 t2)       (in custom elo_tm at level 0).
+Notation "'cr' t1 t2"     := (tm_cr t1 t2)        (in custom elo_tm at level 0).
+Notation "'ptm' tid t"    := (tm_ptm tid t)       (in custom elo_tm at level 0).
+Notation "'spawn' t"      := (tm_spawn t)         (in custom elo_tm at level 0).
 
-Reserved Notation "Gamma '|--' t 'is' T"
-  (at level 40).
+Reserved Notation "Gamma '|--' t 'is' T" (at level 40).
 
-Reserved Notation "'[' x ':=' tx ']' t"
-  (at level 20, x constr, tx at next level, t at next level).
+Reserved Notation "'[' x ':=' tx ']' t" (in custom elo_tm at level 20,
+  x constr).
 
 Reserved Notation "t '--[' e ']-->' t'" (at level 40,
   e at next level).
 
-Reserved Notation "m '--[m' e ']-->' m' " (at level 40,
-  e at next level).
+Reserved Notation "m / t '==[' e ']==>' m' / t'" (at level 40,
+  t at next level, e at next level, m' at next level).
 
-Reserved Notation "m / ts '--[c' tid , e ']-->' m' / ts'" (at level 40,
-  ts at next level,
-  tid at next level, e at next level,
-  m' at next level, ts' at next level).
+Reserved Notation "m / ths '~~[' tid , e ']~~>' m' / ths'" (at level 40,
+  ths at next level, tid at next level, e at next level, m' at next level).
 
-Reserved Notation "m / ts / ls '--[s' tid , e ']-->' m' / ts' / ls' "
-  (at level 40,
-    ts at next level, ls at next level,
-    tid at next level, e at next level,
-    m' at next level, ts' at next level).
-
-Reserved Notation "m / ts / ls '--[' tc ']-->*' m' / ts' / ls' " (at level 40,
-  ts at next level, ls at next level,
-  tc at next level,
-  m' at next level, ts' at next level).
+Reserved Notation "m / ths '~~[' tc ']~~>*' m' / ths' " (at level 40,
+  ths at next level, tc at next level, m' at next level).
 
 (* ------------------------------------------------------------------------- *)
 (* values                                                                    *)
 (* ------------------------------------------------------------------------- *)
 
 Inductive value : tm -> Prop :=
-  | v_unit : value <{ unit }> 
-  | v_num  : forall n, value <{ nat n }>
-  | v_fun  : forall x Tx t, value <{ fn x Tx t }>
-  | v_ref  : forall ad T, value <{ &ad :: T }>
-  | v_mtx  : forall l t, value <{ mtx l t }>
+  | v_unit : value <{unit}>
+  | v_num  : forall n, value <{nat n}>
+  | v_fun  : forall x Tx t, value <{fn x Tx t}> 
+  | v_ref  : forall ad T, value <{&ad : T}>
+  | v_ptm  : forall ad t, value <{ptm ad t}>
   .
 
 (* ------------------------------------------------------------------------- *)
@@ -146,96 +133,111 @@ Inductive value : tm -> Prop :=
 
 Inductive eff : Set :=
   | e_none
-  | e_alloc   (ad : addr) (t : tm) (T : typ)
-  | e_read    (ad : addr) (t : tm)
-  | e_write   (ad : addr) (t : tm) (T : typ)
-  | e_spawn   (t : tm)
-  | e_newlock (l : lock)
-  | e_lock    (l : lock)
-  | e_unlock  (l : lock)
+  | e_alloc (ad : addr) (t : tm) (T : ty)
+  | e_read  (ad : addr) (t : tm)
+  | e_write (ad : addr) (t : tm) (T : ty)
+  | e_spawn (tid : nat) (t : tm)
+  | e_acq   (tid : nat) (ad : addr) (t : tm)
+  | e_rel   (tid : nat) (ad : addr)
   .
+
+(* ------------------------------------------------------------------------- *)
+(* aliases                                                                   *)
+(* ------------------------------------------------------------------------- *)
+
+Definition ctx := map ty.
+
+Definition mem     := list (tm * ty).
+Definition threads := list tm.
+Definition trace   := list (nat * eff).
+
+Definition tm_default  := <{unit}>.
+Definition ty_default  := `Unit`.
+Definition mem_default := (tm_default, ty_default).
+Definition tc_default  := (0, e_none).
 
 (* ------------------------------------------------------------------------- *)
 (* typing                                                                    *)
 (* ------------------------------------------------------------------------- *)
 
-Definition ctx := map typ.
-
 (* Filters out of the context all variables with non-immutable types. *)
 Definition safe (Gamma : ctx) : ctx :=
   fun k => 
     match Gamma k with
-    | Some <{{ Safe T }}> => Some <{{ Safe T }}>
+    | Some `Safe T` => Some `Safe T`
     | _ => None
     end.
 
-Inductive type_of : ctx -> tm -> typ -> Prop :=
+Inductive type_of : ctx -> tm -> ty -> Prop :=
   | T_unit : forall Gamma,
-    Gamma |-- <{ unit }> is <{{ Unit }}>
+    Gamma |-- <{unit}> is `Unit`
 
   | T_num : forall Gamma n,
-    Gamma |-- <{ nat n }> is <{{ Num }}>
+    Gamma |-- <{nat n}> is `Num`
 
   | T_var : forall Gamma x T,
     Gamma x = Some T ->
-    Gamma |-- <{ var x }> is T
+    Gamma |-- <{var x}> is T
 
   | T_fun : forall Gamma x t T Tx,
     Gamma[x <== Tx] |-- t is T ->
-    Gamma |-- <{ fn x Tx t }> is <{{ Tx --> T }}>
+    Gamma |-- <{fn x Tx t}> is `Tx --> T`
 
   | T_call : forall Gamma t1 t2 Tx T,
-    Gamma |-- t1 is <{{ Tx --> T }}> ->
+    Gamma |-- t1 is `Tx --> T` ->
     Gamma |-- t2 is Tx ->
-    Gamma |-- <{ call t1 t2 }> is T
+    Gamma |-- <{call t1 t2}> is T
 
-  | T_refU : forall Gamma ad T,
-    Gamma |-- <{ &ad :: u&T }> is <{{ u&T }}>
+  | T_refR : forall Gamma ad T,
+    Gamma |-- <{&ad : r&T}> is `r&T`
 
-  | T_refS : forall Gamma ad T,
-    Gamma |-- <{ &ad :: s&T }> is <{{ s&T }}>
+  | T_refX : forall Gamma ad T,
+    Gamma |-- <{&ad : x&T}> is `x&T`
 
-  | T_newU : forall Gamma t T,
+  | T_refW : forall Gamma ad T,
+    Gamma |-- <{&ad : w&T}> is `w&T`
+
+  | T_newR : forall Gamma t T,
+    Gamma |-- t is `Safe T` ->
+    Gamma |-- <{new t : r&T}> is `r&T`
+
+  | T_newX : forall Gamma t T,
+    safe Gamma |-- t is T ->
+    Gamma |-- <{new t : x&T}> is `x&T`
+
+  | T_newW : forall Gamma t T,
     Gamma |-- t is T ->
-    Gamma |-- <{ new u&T t }> is <{{ u&T }}>
+    Gamma |-- <{new t : w&T}> is `w&T`
 
-  | T_newS : forall Gamma t T,
-    Gamma |-- t is <{{ Safe T }}> ->
-    Gamma |-- <{ new s&T t }> is <{{ s&T }}>
+  | T_loadR : forall Gamma t T,
+    Gamma |-- t is `r&T` ->
+    Gamma |-- <{*t}> is `Safe T`
 
-  | T_loadU : forall Gamma t T,
-    Gamma |-- t is <{{ u&T }}> ->
-    Gamma |-- <{ *t }> is T
-
-  | T_loadS : forall Gamma t T,
-    Gamma |-- t is <{{ s&T }}> ->
-    Gamma |-- <{ *t }> is <{{ Safe T }}>
+  | T_loadW : forall Gamma t T,
+    Gamma |-- t is `w&T` ->
+    Gamma |-- <{*t}> is T
 
   | T_asg : forall Gamma t1 t2 T,
-    Gamma |-- t1 is <{{ u&T }}> ->
+    Gamma |-- t1 is `w&T` ->
     Gamma |-- t2 is T ->
-    Gamma |-- <{ t1 = t2 }> is <{{ Unit }}>
+    Gamma |-- <{t1 := t2}> is `Unit`
+
+  | T_acq : forall Gamma t1 t2 T1 T2,
+    Gamma |-- t1 is `x&T1` ->
+    safe Gamma |-- t2 is `T1 --> Safe T2` ->
+    Gamma |-- <{acq t1 t2}> is `Safe T2`
+
+  | T_cr : forall Gamma ad t T,
+    empty |-- t is T ->
+    Gamma |-- <{cr ad t}> is T
+
+  | T_ptm : forall Gamma tid t T,
+    empty |-- t is T ->
+    Gamma |-- <{ptm tid t}> is T
 
   | T_spawn : forall Gamma t T,
     safe Gamma |-- t is T ->
-    Gamma |-- <{ spawn t }> is <{{ Unit }}> 
-
-  | T_mtx : forall Gamma l t T,
-    empty |-- t is T -> (* TODO *)
-    Gamma |-- <{ mtx l t }> is <{{ Mtx T }}>
-
-  | T_newx : forall Gamma t T,
-    safe Gamma |-- t is T ->
-    Gamma |-- <{ newx t }> is <{{ Mtx T }}>
-
-  | T_acq : forall Gamma t1 t2 T1 T2,
-    Gamma |-- t1 is <{{ Mtx T1 }}> ->
-    safe Gamma |-- t2 is <{{ T1 --> Safe T2 }}> ->
-    Gamma |-- <{ acq t1 t2 }> is <{{ Safe T2 }}>
-
-  | T_cr : forall Gamma l t T,
-    empty |-- t is T -> (* TODO *)
-    Gamma |-- <{ cr l t }> is T
+    Gamma |-- <{spawn t}> is `Unit` 
 
   where "Gamma '|--' t 'is' T" := (type_of Gamma t T).
 
@@ -247,23 +249,24 @@ Local Infix "=?" := string_dec (at level 70, no associativity).
 
 Fixpoint subst (x : id) (tx t : tm) : tm :=
   match t with
-  | <{ unit        }> => t
-  | <{ nat _       }> => t
-  | <{ & _ :: _    }> => t
-  | <{ new T t'    }> => <{ new T ([x := tx] t')            }>
-  | <{ *t'         }> => <{ * ([x := tx] t')                }>
-  | <{ t1 = t2     }> => <{ ([x := tx] t1) = ([x := tx] t2) }>
-  | <{ var x'      }> => if x =? x' then tx else t
-  | <{ fn x' Tx t' }> => if x =? x' then t  else <{ fn x' Tx ([x := tx] t') }>
-  | <{ call t1 t2  }> => <{ call ([x := tx] t1) ([x := tx] t2) }>
-  | <{ spawn t'    }> => <{ spawn ([x := tx] t')               }>
-  (* TODO *)
-  | tm_mtx  _ _ => <{ unit }>
-  | tm_newx _   => <{ unit }>
-  | tm_acq  _ _ => <{ unit }>
-  | tm_cr   _ _ => <{ unit }>
+  | <{unit       }> => t
+  | <{nat _      }> => t
+  (* functions *)
+  | <{var x'     }> => if x =? x' then tx else t
+  | <{fn x' Tx t'}> => if x =? x' then t  else <{fn x' Tx ([x := tx] t')}>
+  (* memory *)
+  | <{call t1 t2 }> => <{call ([x := tx] t1) ([x := tx] t2)}>
+  | <{& _ : _    }> => t
+  | <{new t' : T }> => <{new ([x := tx] t') : T}>
+  | <{*t'        }> => <{* ([x := tx] t')}>
+  | <{t1 := t2   }> => <{([x := tx] t1) := ([x := tx] t2)}>
+  | <{acq t1 t2  }> => <{acq ([x := tx] t1) ([x := tx] t2)}>
+  | <{cr ad t'   }> => <{cr ad ([x := tx] t')}> (* could it be "t"? *)
+  | <{ptm _ _    }> => t
+  (* concurrency *)
+  | <{spawn t'   }> => <{spawn ([x := tx] t')}>
   end
-  where "'[' x ':=' tx ']' t" := (subst x tx t).
+  where "'[' x ':=' tx ']' t" := (subst x tx t) (in custom elo_tm).
 
 (* ------------------------------------------------------------------------- *)
 (* operational semantics -- term step                                        *)
@@ -273,82 +276,81 @@ Inductive tstep : tm -> eff -> tm -> Prop :=
   (* Call *)
   | ts_call1 : forall t1 t1' t2 e,
     t1 --[e]--> t1' ->
-    <{ call t1 t2 }> --[e]--> <{ call t1' t2 }>
+    <{call t1 t2}> --[e]--> <{call t1' t2}>
 
   | ts_call2 : forall t1 t2 t2' e,
     value t1 ->
     t2 --[e]--> t2' ->
-    <{ call t1 t2 }> --[e]--> <{ call t1 t2' }>
+    <{call t1 t2}> --[e]--> <{call t1 t2'}>
 
   | ts_call : forall x Tx t tx,
     value tx ->
-    <{ call {fn x Tx t} tx }> --[e_none]--> ([x := tx] t)
+    <{call (fn x Tx t) tx}> --[e_none]--> <{[x := tx] t}>
 
   (* New *)
   | ts_new1 : forall t t' e T,
     t --[e]--> t' ->
-    <{ new T t }> --[e]--> <{ new T t' }>
+    <{new t : T}> --[e]--> <{new t' : T}>
 
-  | ts_new : forall ad t T,
+  | ts_newR : forall ad t T,
     value t ->
-    <{ new T t }> --[e_alloc ad t T]--> <{ &ad :: T }>
+    <{new t : r&T}>  --[e_alloc ad t `r&T`]--> <{&ad : r&T}>
+
+  | ts_newX : forall ad t T,
+    value t ->
+    <{new t : x&T}> --[e_alloc ad <{ptm None t}> `x&T`]--> <{&ad : x&T}>
+
+  | ts_newW : forall ad t T,
+    value t ->
+    <{new t : w&T}> --[e_alloc ad t `w&T`]--> <{&ad : w&T}>
 
   (* Load *)
   | ts_load1 : forall t t' e,
     t --[e]--> t' ->
-    <{ *t }> --[e]--> <{ *t' }>
+    <{*t}> --[e]--> <{*t'}>
 
   | ts_load : forall ad t T,
-    <{ * &ad :: T }> --[e_read ad t]--> t
+    <{* (&ad : T)}> --[e_read ad t]--> t
 
   (* Asg *)
   | ts_asg1 : forall t1 t1' t2 e,
     t1 --[e]--> t1' ->
-    <{ t1 = t2 }> --[e]--> <{ t1' = t2 }>
+    <{t1 := t2}> --[e]--> <{t1' := t2}>
 
   | ts_asg2 : forall t1 t2 t2' e,
     value t1 ->
     t2 --[e]--> t2' ->
-    <{ t1 = t2 }> --[e]--> <{ t1 = t2' }>
+    <{t1 := t2}> --[e]--> <{t1 := t2'}>
 
   | ts_asg : forall ad t T,
     value t ->
-    <{ {&ad :: T} = t }> --[e_write ad t T]--> <{ unit }>
-
-  (* Spawn *)
-  | ts_spawn : forall t,
-    <{ spawn t }> --[e_spawn t]--> <{ unit }>
-
-  (* New Mutex *)
-  | ts_newx1 : forall t t' e,
-    t --[e]--> t' ->
-    <{ newx t }> --[e]--> <{ newx t' }>
-
-  | ts_newx : forall t l,
-    value t ->
-    <{ newx t }> --[e_newlock l]--> <{ mtx l t }>
+    <{&ad : T := t}> --[e_write ad t T]--> <{unit}>
 
   (* Acquire *)
   | ts_acq1 : forall t1 t1' t2 e,
     t1 --[e]--> t1' ->
-    <{ acq t1 t2 }> --[e]--> <{ acq t1' t2 }>
+    <{acq t1 t2}> --[e]--> <{acq t1' t2}>
 
   | ts_acq2 : forall t1 t2 t2' e,
     value t1 ->
     t2 --[e]--> t2' ->
-    <{ acq t1 t2 }> --[e]--> <{ acq t1 t2' }>
+    <{acq t1 t2}> --[e]--> <{acq t1 t2'}>
 
-  | ts_acq : forall l x Tx t tx,
-    <{ acq {mtx l tx} {fn x Tx t} }> --[e_lock l]--> <{ cr l ([x := tx] t) }>
+  | ts_acq : forall tid ad T x Tx t tx,
+    <{acq (&ad : T) (fn x Tx t)}> --[e_acq tid ad tx]--> <{cr ad ([x := tx] t)}>
 
   (* Critical Region *)
-  | ts_cr1 : forall l t t' e,
+  | ts_cr1 : forall ad t t' e,
     t --[e]--> t' ->
-    <{ cr l t }> --[e]--> <{ cr l t' }>
+    <{cr ad t}> --[e]--> <{cr ad t'}>
 
-  | ts_cr : forall l t,
+  | ts_cr : forall tid ad t,
     value t ->
-    <{ cr l t }> --[e_unlock l]--> t
+    <{cr ad t}> --[e_rel tid ad]--> t
+
+  (* Spawn *)
+  | ts_spawn : forall tid t,
+    <{spawn t}> --[e_spawn tid t]--> <{unit}>
 
   where "t '--[' e ']-->' t'" := (tstep t e t').
 
@@ -356,102 +358,81 @@ Inductive tstep : tm -> eff -> tm -> Prop :=
 (* operational semantics -- memory step                                      *)
 (* ------------------------------------------------------------------------- *)
 
-Definition mem := list (tm * typ).
-Definition memory_default := (<{ unit }>, <{{ Unit }}>).
+Notation " ths '[' tid ']' " := (ths[tid] or tm_default)
+  (at level 9, tid at next level).
 
-Notation " l '[' i '].tm' " := (fst (l[i] or memory_default))
-  (at level 9, i at next level).
-Notation " l '[' i '].ty' " := (snd (l[i] or memory_default))
-  (at level 9, i at next level).
+Notation " m '[' ad '].tm' " := (fst (m[ad] or mem_default))
+  (at level 9, ad at next level).
 
-Inductive mstep : mem -> eff -> mem -> Prop :=
-  | ms_alloc : forall m t T,
-    m --[m e_alloc (#m) t T]--> (m +++ (t, T))
+Notation " m '[' ad '].ty' " := (snd (m[ad] or mem_default))
+  (at level 9, ad at next level).
 
-  | ms_read : forall m ad,
+Inductive mstep : mem -> tm -> eff -> mem -> tm -> Prop :=
+  | ms_none : forall m t t',
+    t --[e_none]--> t' ->
+    m / t ==[e_none]==> m / t'
+
+  | ms_alloc : forall m t t' ad te T,
+    ad = #m ->
+    t --[e_alloc ad te T]--> t' ->
+    m / t ==[e_alloc ad te T]==> (m +++ (te, T)) / t'
+
+  | ms_read : forall m t t' ad te,
     ad < #m ->
-    m --[m e_read ad m[ad].tm]--> m
+    te = m[ad].tm ->
+    t --[e_read ad te]--> t' ->
+    m / t ==[e_read ad te]==> m / t'
 
-  | ms_write : forall m ad te T,
+  | ms_write : forall m t t' ad te T,
     ad < #m ->
-    m --[m e_write ad te T]--> m[ad <- (te, T)]
+    t --[e_write ad te T]--> t' ->
+    m / t ==[e_write ad te T]==> m[ad <- (te, T)] / t'
 
-  where "m '--[m' e ']-->' m' " := (mstep m e m').
+  | ms_acq : forall m t t' tid ad te T,
+    ad < #m ->
+    m[ad].tm = <{ptm None te}> ->
+    m[ad].ty = T ->
+    t --[e_acq tid ad te]--> t' ->
+    m / t ==[e_acq tid ad te]==> m[ad <- (tm_ptm (Some tid) te, T)] / t'
+
+  | ms_rel : forall m t t' te tid ad T,
+    ad < #m ->
+    m[ad].tm = tm_ptm (Some tid) te ->
+    m[ad].ty = T ->
+    t --[e_rel tid ad]--> t' ->
+    m / t ==[e_rel tid ad]==> m[ad <- (tm_ptm None te, T)] / t'
+
+  where "m / t '==[' e ']==>' m' / t'" := (mstep m t e m' t').
 
 (* ------------------------------------------------------------------------- *)
-(* operational semantics -- concurrent step                                  *)
+(* operational semantics -- step                                             *)
 (* ------------------------------------------------------------------------- *)
-
-Definition threads := list tm.
-Definition thread_default := <{ unit }>.
-
-Notation " l '[' i ']' " := (l[i] or thread_default)
-  (at level 9, i at next level).
 
 Inductive cstep : mem -> threads -> nat -> eff -> mem -> threads -> Prop :=
-  | cs_spawn : forall m ts t' tid te,
-      tid < #ts ->
-      ts[tid] --[e_spawn te]--> t' ->
-      m / ts --[c tid, e_spawn te]--> m / (ts[tid <- t'] +++ te)
+  | cs_mem : forall m m' t' ths tid e,
+    tid < #ths ->
+    m / ths[tid] ==[e]==> m' / t' ->
+    m / ths ~~[tid, e]~~> m' / ths[tid <- t']
 
-  | cs_mem : forall m m' ts t' tid e,
-      tid < #ts ->
-      m / ts[tid] --[m e]--> m' / t' ->
-      m / ts --[c tid, e]--> m' / ts[tid <- t']
+  | cs_spawn : forall m t' te ths tid e,
+    tid < #ths ->
+    ths[tid] --[e_spawn (#ths) te]--> t' ->
+    m / ths ~~[tid, e]~~> m / (ths[tid <- t'] +++ te)
 
-    where "m / ts '--[c' tid ,  e ']-->' m' / ts'" :=
-      (cstep m ts tid e m' ts').
-
-(* ------------------------------------------------------------------------- *)
-(* operational semantics -- sync step                                        *)
-(* ------------------------------------------------------------------------- *)
-
-Definition locks := list (option nat).
-
-Inductive sstep :
-  mem -> threads -> locks -> nat -> eff -> mem -> threads -> locks -> Prop :=
-
-  | ss_newlock : forall m m' ls ts ts' tid l,
-    l = #ls ->
-    m / ts --[c tid, e_newlock l]--> m' / ts' ->
-    m / ts / ls --[s tid, e_newlock l]--> m / ts' / (ls +++ None)
-
-  | ss_lock : forall m m' ls ts ts' tid l,
-    l < #ls ->
-    ls[l] or None = None ->
-    m / ts --[c tid, e_lock l]--> m' / ts' ->
-    m / ts / ls --[s tid, e_lock l]--> m / ts' / ls[l <- Some tid]
-
-  | ss_unlock : forall m m' ls ts ts' tid l,
-    l < #ls ->
-    ls[l] or None = Some tid ->
-    m / ts --[c tid, e_unlock l]--> m' / ts' ->
-    m / ts / ls --[s tid, e_unlock l]--> m / ts' / ls[l <- None]
-
-  | ss_conc : forall m m' ls ts ts' tid e,
-    m / ts --[c tid, e]--> m' / ts' ->
-    m / ts / ls --[s tid, e]--> m' / ts' / ls
-
-  where "m / ls / ts '--[s' tid , e ']-->' m' / ls' / ts'" :=
-    (sstep m ls ts tid e m' ls' ts').
+  where "m / ths '~~[' tid , e ']~~>' m' / ths'" := (cstep m ths tid e m' ths').
 
 (* ------------------------------------------------------------------------- *)
 (* multistep                                                                 *)
 (* ------------------------------------------------------------------------- *)
 
-Definition trace := list (nat * eff).
+Inductive multistep : mem -> threads -> trace -> mem -> threads -> Prop :=
+  | multistep_refl: forall m ths,
+    m / ths ~~[nil]~~>* m / ths
 
-Inductive multistep :
-  mem -> threads -> locks -> trace -> mem -> threads -> locks -> Prop :=
+  | multistep_trans : forall m m' m'' ths ths' ths'' tid e tc,
+    m  / ths  ~~[tc            ]~~>* m'  / ths'  ->
+    m' / ths' ~~[tid, e        ]~~>  m'' / ths'' ->
+    m  / ths  ~~[(tid, e) :: tc]~~>* m'' / ths'' 
 
-  | multistep_refl: forall m ls ts,
-    m / ls / ts --[nil]-->* m / ls / ts
-
-  | multistep_trans : forall m m' m'' ts ts' ts'' ls ls' ls'' tid e tc,
-    m  / ts  / ls  --[tc            ]-->* m'  / ts'  / ls'  ->
-    m' / ts' / ls' --[s tid, e      ]-->  m'' / ts'' / ls'' ->
-    m  / ts  / ls  --[(tid, e) :: tc]-->* m'' / ts'' / ls'' 
-
-  where "m / ts / ls '--[' tc ']-->*' m' / ts' / ls'" :=
-    (multistep m ts ls tc m' ts' ls').
+  where "m / ths '~~[' tc ']~~>*' m' / ths'" := (multistep m ths tc m' ths').
 
