Constructors.v
@@ -3,6 +3,96 @@ From Elo Require Import Definitions.
 From Elo Require Import Inversions.
 
 (* ------------------------------------------------------------------------- *)
+(* not-write-access constructors                                             *)
+(* ------------------------------------------------------------------------- *)
+
+Local Ltac solve_nwacc_construction :=
+  intros ** ?; invc_wacc; contradiction.
+
+Lemma nwacc_unit : forall m ad,
+  ~ write_access ad m <{unit}>.
+Proof.
+  solve_nwacc_construction.
+Qed.
+
+Lemma nwacc_nat : forall m ad n,
+  ~ write_access ad m <{nat n}>.
+Proof. solve_nwacc_construction. Qed.
+
+Lemma nwacc_fun : forall m x Tx t ad,
+  ~ write_access ad m t ->
+  ~ write_access ad m <{fn x Tx t}>.
+Proof. solve_nwacc_construction. Qed.
+
+Lemma nwacc_call : forall m t1 t2 ad,
+  ~ write_access ad m t1 ->
+  ~ write_access ad m t2 ->
+  ~ write_access ad m <{call t1 t2}>.
+Proof. solve_nwacc_construction. Qed.
+
+Lemma nwacc_refS : forall m ad ad' T,
+  ~ write_access ad m <{&ad' :: s&T}>.
+Proof. solve_nwacc_construction. Qed.
+
+Lemma nwacc_refX : forall m ad ad' T,
+  ~ write_access ad m <{&ad' :: x&T}>.
+Proof. solve_nwacc_construction. Qed.
+
+(*
+Lemma nacc_ref : forall m ad ad' T,
+  ad <> ad' ->
+  ~ access ad m m[ad'].tm ->
+  ~ access ad m <{&ad' :: T}>.
+Proof. solve_nacc_construction. Qed.
+*)
+
+Lemma nwacc_new : forall m t ad T,
+  ~ write_access ad m t ->
+  ~ write_access ad m <{new T t}>.
+Proof. solve_nwacc_construction. Qed.
+
+Lemma nwacc_load : forall m t ad,
+  ~ write_access ad m t ->
+  ~ write_access ad m <{*t}>.
+Proof. solve_nwacc_construction. Qed.
+
+Lemma nwacc_asg : forall m t1 t2 ad,
+  ~ write_access ad m t1 ->
+  ~ write_access ad m t2 ->
+  ~ write_access ad m <{t1 = t2}>.
+Proof. solve_nwacc_construction. Qed.
+
+Lemma nwacc_acq : forall m t1 t2 ad,
+  ~ write_access ad m t1 ->
+  ~ write_access ad m t2 ->
+  ~ write_access ad m <{acq t1 t2}>.
+Proof. solve_nwacc_construction. Qed.
+
+Lemma nwacc_cr : forall m t ad ad',
+  ~ write_access ad m t ->
+  ~ write_access ad m <{cr ad' t}>.
+Proof. solve_nwacc_construction. Qed.
+
+Lemma nwacc_ptm : forall m t ad tid,
+  ~ write_access ad m t ->
+  ~ write_access ad m <{ptm tid t}>.
+Proof. solve_nwacc_construction. Qed.
+
+Lemma nwacc_spawn : forall m t ad,
+  ~ write_access ad m <{spawn t}>.
+Proof. solve_nwacc_construction. Qed.
+
+#[export] Hint Resolve
+  nwacc_unit  nwacc_nat
+  nwacc_fun   nwacc_call
+  nwacc_refS  nwacc_refX
+  nwacc_new   nwacc_load nwacc_asg
+  nwacc_acq   nwacc_cr   nwacc_ptm
+  nwacc_spawn
+  : wacc.
+
+(*
+(* ------------------------------------------------------------------------- *)
 (* not-access constructors                                                   *)
 (* ------------------------------------------------------------------------- *)
 
@@ -69,4 +159,4 @@ Proof. solve_nacc_construction. Qed.
   nacc_seq
   nacc_spawn
   : acc.
-
+*)
