Core.v
@@ -2,5 +2,5 @@ From Elo Require Export Util.
 From Elo Require Export Array.
 From Elo Require Export Map.
 From Elo Require Export Sem.
-From Elo Require Export Ext.
+From Elo Require Export SemExt.
 
