HappensBefore.v
@@ -1,0 +1,31 @@
+From Coq Require Import Lia.
+From Coq Require Import Lists.List.
+
+From Elo Require Import Core.
+
+
+Theorem always_happens_before : forall m m' ths ,
+  m / ths ~~[tc]~~>* m' / ths' ->
+  tc[evA] = (tid1, e_write ad v1 T1) ->
+  tc[evB] = (tid2, e_write ad v2 T2) ->
+  evA < evB ->
+  evA << evB in tc.
+Proof.
+Abort.
+
+Theorem always_happens_before :
+  forall mA mX mY mB thsA thsX thsY thsB tid1 tid2 ad v1 v2 tc T,
+    mA / thsA ~~[ tid1, e_write ad v1 T ]~~>  mX / thsX ->
+    mX / thsX ~~[ tc                    ]~~>* mY / thsY ->
+    mY / thsY ~~[ tid2, e_read ad v2    ]~~>  mB / thsB ->
+    0 << (#tc + 1) in
+      ((tid2, e_read ad v2) :: tc ++ (tid1, e_write ad v1 T) :: nil).
+Proof.
+  intros. destruct (nat_eq_dec tid1 tid2); subst.
+  - eapply hb_thread.
+    + lia.
+    + clear H. clear H0. clear H1.
+      simpl. induction tc.
+      * eauto.
+      * simpl in *.
+Qed.
