Preservation.v
@@ -1,11 +1,7 @@
-From Coq Require Import Lia.
-
 From Elo Require Import Core.
 From Elo Require Import Properties.
-From Elo Require Import PtrTyp.
-From Elo Require Import Lemmas.
-From Elo Require Import Generic.
-From Elo Require Import Inheritance.
+
+From Elo Require Import SimpleLemmas.
 
 (* simpl forall-threads *)
 Ltac simplfths := 
@@ -27,7 +23,7 @@ Ltac split_preservation :=
     _ : ?m1 / ?ths1 ~~[_, _]~~> ?m2 / ?ths2
      |- forall_program ?m2 ?ths2 (?P ?m2) =>
     destruct_forall_program;
-    invc_cstep; try invc_mstep; split; try simplfths; trivial
+    invc_cstep; try invc_mstep; trivial; split; try simplfths; trivial
   (* ss *)
   | H : forall_program ?m1 ?ths1 ?P,
     _ : ?m1 / ?ths1 ~~[_, _]~~> ?m2 / ?ths2
@@ -57,9 +53,10 @@ Theorem value_preservation : forall m m' ths ths' tid e,
   m / ths ~~[tid, e]~~> m' / ths' ->
   forall_memory m' value.
 Proof.
-  assert (forall t t' ad v T, t --[EF_Alloc ad v T]--> t' -> value v);
-  assert (forall t t' ad v T, t --[EF_Write ad v T]--> t' -> value v);
-  try solve [intros; induction_tstep; eauto].
+  assert (forall t t' ad te T, t --[e_alloc ad te T]--> t' -> value te)
+    by (intros; ind_tstep; eauto using value). 
+  assert (forall t t' ad te T, t --[e_write ad te T]--> t' -> value te)
+    by (intros; ind_tstep; eauto). 
   intros. inv_cstep; trivial. inv_mstep; trivial;
   (eapply forall_array_add || eapply forall_array_set); eauto using value.
 Qed.
@@ -68,138 +65,239 @@ Qed.
 (* valid-addresses                                                           *)
 (* ------------------------------------------------------------------------- *)
 
-Lemma vad_subst : forall m t v x,
-  valid_addresses m v ->
+Lemma vad_subst : forall m t tx x,
+  valid_addresses m tx ->
   valid_addresses m t ->
-  valid_addresses m ([x := v]t).
+  valid_addresses m <{[x := tx] t}>.
 Proof.
-  intros. induction t; try inv_vad; eauto using valid_addresses;
-  simpl; destruct string_eq_dec; eauto using valid_addresses.
+  intros.
+  induction t; try inv_vad; eauto using valid_addresses;
+  simpl; destruct str_eq_dec; eauto using valid_addresses.
 Qed.
 
-Lemma vad_mem_add : forall m t vT,
+Lemma vad_mem_add : forall m t tT,
   valid_addresses m t ->
-  valid_addresses (m +++ vT) t.
+  valid_addresses (m +++ tT) t.
 Proof.
   intros.
   induction t; try inv_vad; eauto using valid_addresses.
   eapply vad_ref. rewrite add_increments_length. eauto.
 Qed.
 
-Lemma vad_mem_set : forall m t ad vT,
+Lemma vad_mem_set : forall m t ad tT,
   valid_addresses m t ->
-  valid_addresses m[ad <- vT] t.
+  valid_addresses m[ad <- tT] t.
 Proof.
   intros.
   induction t; try inv_vad; eauto using valid_addresses.
   eapply vad_ref. rewrite set_preserves_length. assumption.
 Qed.
 
-(* ------------------------------------------------------------------------- *)
+Local Lemma vad_ptm : forall m otid1 otid2 ad t T,
+  forall_memory m (valid_addresses m) ->
+  m[ad].tm = <{ptm otid1 t}> ->
+  valid_addresses m[ad <- (<{ptm otid2 t}>, T)] t.
+Proof.
+  intros * Hmvad Hptm.
+  specialize (Hmvad ad). simpl in Hmvad.
+  rewrite Hptm in Hmvad. invc_vad. eauto using vad_mem_set.
+Qed.
+
+(* none -------------------------------------------------------------------- *)
 
 Lemma vad_preservation_none : forall m t1 t2,
   valid_addresses m t1 ->
-  t1 --[EF_None]--> t2 ->
+  t1 --[e_none]--> t2 ->
   valid_addresses m t2.
 Proof.
   intros.
-  induction_tstep; inv_vad; eauto using valid_addresses.
-  inv_vad. eauto using (must_subst valid_addresses).
+  ind_tstep; inv_vad; eauto using valid_addresses.
+  inv_vad. eauto using vad_subst.
 Qed.
 
-(* ------------------------------------------------------------------------- *)
+(* alloc ------------------------------------------------------------------- *)
 
-Lemma vad_preservation_mem_alloc : forall m t1 t2 v T,
+Lemma vad_preservation_mem_alloc : forall m t1 t2 t T,
   valid_addresses m t1 ->
   (* --- *)
   forall_memory m (valid_addresses m) ->
-  t1 --[EF_Alloc (#m) v T]--> t2 ->
-  forall_memory (m +++ (v, T)) (valid_addresses (m +++ (v, T))).
+  t1 --[e_alloc (#m) t T]--> t2 ->
+  forall_memory (m +++ (t, T)) (valid_addresses (m +++ (t, T))).
 Proof.
   intros.
-  induction_tstep; inv_vad; eauto. 
-  intros ad'. Array.sga; eauto using vad_mem_add, valid_addresses.
+  ind_tstep; inv_vad; eauto;
+  intros ?; Array.sga; eauto using vad_mem_add, valid_addresses.
 Qed.
 
-Lemma vad_preservation_alloc : forall m t1 t2 v T,
+Lemma vad_preservation_alloc : forall m t1 t2 t T,
   valid_addresses m t1 ->
-  t1 --[EF_Alloc (#m) v T]--> t2 ->
-  valid_addresses (m +++ (v, T)) t2.
+  t1 --[e_alloc (#m) t T]--> t2 ->
+  valid_addresses (m +++ (t, T)) t2.
 Proof.
   intros.
-  induction_tstep; inv_vad; eauto using vad_mem_add, valid_addresses.
-  eapply vad_ref. rewrite add_increments_length. eauto.
+  ind_tstep; inv_vad; eauto using vad_mem_add, valid_addresses;
+  eapply vad_ref; rewrite add_increments_length; eauto.
 Qed.
 
-Lemma vad_preservation_unt_alloc : forall m t1 t2 t ad v T,
+Lemma vad_preservation_unt_alloc : forall m t1 t2 t ad te T,
   valid_addresses m t ->
-  t1 --[EF_Alloc ad v T]--> t2 ->
-  valid_addresses (m +++ (v, T)) t.
+  t1 --[e_alloc ad te T]--> t2 ->
+  valid_addresses (m +++ (te, T)) t.
 Proof.
   eauto using vad_mem_add.
 Qed.
 
-(* ------------------------------------------------------------------------- *)
+(* read -------------------------------------------------------------------- *)
 
 Lemma vad_preservation_read : forall m t1 t2 ad,
   forall_memory m (valid_addresses m) ->
   (* --- *)
   valid_addresses m t1 ->
-  t1 --[EF_Read ad m[ad].tm]--> t2 ->
+  t1 --[e_read ad m[ad].tm]--> t2 ->
   valid_addresses m t2.
 Proof.
   intros.
-  induction_tstep; inv_vad; eauto using valid_addresses.
+  ind_tstep; inv_vad; eauto using valid_addresses.
 Qed.
 
-(* ------------------------------------------------------------------------- *)
+(* write ------------------------------------------------------------------- *)
 
-Lemma vad_preservation_mem_write : forall m t1 t2 ad v T,
+Lemma vad_preservation_mem_write : forall m t1 t2 ad te T,
   valid_addresses m t1 ->
   (* --- *)
   ad < #m ->
   forall_memory m (valid_addresses m) ->
-  t1 --[EF_Write ad v T]--> t2 ->
-  forall_memory m[ad <- (v, T)] (valid_addresses m[ad <- (v, T)]).
+  t1 --[e_write ad te T]--> t2 ->
+  forall_memory m[ad <- (te, T)] (valid_addresses m[ad <- (te, T)]).
 Proof.
   intros.
-  induction_tstep; inv_vad; eauto. 
+  ind_tstep; inv_vad; eauto. 
   intros ad'. Array.sgs; eauto using vad_mem_set.
 Qed.
 
-Lemma vad_preservation_write : forall m t1 t2 ad v T,
+Lemma vad_preservation_write : forall m t1 t2 ad t T,
   valid_addresses m t1 ->
-  t1 --[EF_Write ad v T]--> t2 ->
-  valid_addresses (m[ad <- (v, T)]) t2.
+  t1 --[e_write ad t T]--> t2 ->
+  valid_addresses (m[ad <- (t, T)]) t2.
 Proof.
   intros.
-  induction_tstep; inv_vad; eauto using vad_mem_set, valid_addresses.
+  ind_tstep; inv_vad; eauto using vad_mem_set, valid_addresses.
 Qed.
 
-Lemma vad_preservation_unt_write : forall m t1 t2 t ad v T,
-  valid_addresses m t ->
-  t1 --[EF_Write ad v T]--> t2 ->
-  valid_addresses m[ad <- (v, T)] t.
+Lemma vad_preservation_unt_write : forall m t1 t2 tu ad t T,
+  valid_addresses m tu ->
+  t1 --[e_write ad t T]--> t2 ->
+  valid_addresses m[ad <- (t, T)] tu.
 Proof.
   eauto using vad_mem_set.
 Qed.
 
-(* ------------------------------------------------------------------------- *)
+(* acq --------------------------------------------------------------------- *)
 
-Lemma vad_preservation_spawn : forall m t1 t2 t,
-  valid_addresses m t1 ->
-  t1 --[EF_Spawn t]--> t2 ->
-  valid_addresses m t2.
+Lemma vad_preservation_mem_acq : forall m1 m2 t1 t2 otid1 otid2 t tid ad T,
+  valid_addresses m1 t1 ->
+  (* --- *)
+  ad < #m1 ->
+  m1[ad].tm = <{ptm otid1 t}> ->
+  m2 = m1[ad <- (<{ptm otid2 t}>, T)] ->
+  (* --- *)
+  forall_memory m1 (valid_addresses m1) ->
+  t1 --[e_acq tid ad t]--> t2 ->
+  forall_memory m2 (valid_addresses m2).
 Proof.
-  intros. induction_tstep; inv_vad; eauto using valid_addresses.
+  intros.
+  ind_tstep; invc_vad; eauto. 
+  intros ad'. Array.sgs; eauto using vad_mem_set, vad_ptm, valid_addresses.
 Qed.
 
-Lemma vad_preservation_spawned : forall m t1 t2 t,
+Lemma vad_preservation_acq : forall m t1 t2 otid1 otid2 t tid ad T,
+  forall_memory m (valid_addresses m) ->
+  (* --- *)
+  ad < #m ->
+  m[ad].tm = <{ptm otid1 t}> ->
+  (* --- *)
   valid_addresses m t1 ->
-  t1 --[EF_Spawn t]--> t2 ->
+  t1 --[e_acq tid ad t]--> t2 ->
+  valid_addresses m[ad <- (<{ptm otid2 t}>, T)] t2.
+Proof.
+  intros.
+  ind_tstep; inv_vad; eauto using vad_mem_set, valid_addresses.
+  repeat invc_vad. eauto using vad_subst, vad_mem_set, vad_ptm, valid_addresses.
+Qed.
+
+Lemma vad_preservation_unt_acq : forall m t1 t2 tu otid1 otid2 t tid ad T,
+  forall_memory m (valid_addresses m) ->
+  (* --- *)
+  ad < #m ->
+  m[ad].tm = <{ptm otid1 t}> ->
+  (* --- *)
+  valid_addresses m tu ->
+  t1 --[e_acq tid ad t]--> t2 ->
+  valid_addresses m[ad <- (<{ptm otid2 t}>, T)] tu.
+Proof.
+  eauto using vad_mem_set.
+Qed.
+
+(* rel --------------------------------------------------------------------- *)
+
+Lemma vad_preservation_mem_rel : forall m m' t1 t2 otid1 otid2 t tid ad T,
+  valid_addresses m t1 ->
+  (* --- *)
+  ad < #m ->
+  m[ad].tm = <{ptm otid1 t}> ->
+  m' = m[ad <- (<{ptm otid2 t}>, T)] ->
+  (* --- *)
+  forall_memory m (valid_addresses m) ->
+  t1 --[e_rel tid ad]--> t2 ->
+  forall_memory m' (valid_addresses m').
+Proof.
+  intros. ind_tstep; invc_vad; eauto. 
+  intros ?. Array.sgs; eauto using vad_mem_set, vad_ptm, valid_addresses.
+Qed.
+
+Lemma vad_preservation_rel : forall m t1 t2 otid1 otid2 t tid ad T,
+  forall_memory m (valid_addresses m) ->
+  (* --- *)
+  ad < #m ->
+  m[ad].tm = <{ptm otid1 t}> ->
+  (* --- *)
+  valid_addresses m t1 ->
+  t1 --[e_rel tid ad]--> t2 ->
+  valid_addresses m[ad <- (<{ptm otid2 t}>, T)] t2.
+Proof.
+  intros.
+  ind_tstep; inv_vad; eauto using vad_mem_set, valid_addresses.
+Qed.
+
+Lemma vad_preservation_unt_rel : forall m t1 t2 tu otid1 otid2 t tid ad T,
+  forall_memory m (valid_addresses m) ->
+  (* --- *)
+  ad < #m ->
+  m[ad].tm = <{ptm otid1 t}> ->
+  (* --- *)
+  valid_addresses m tu ->
+  t1 --[e_rel tid ad]--> t2 ->
+  valid_addresses m[ad <- (<{ptm otid2 t}>, T)] tu.
+Proof.
+  eauto using vad_mem_set.
+Qed.
+
+(* spawn ------------------------------------------------------------------- *)
+
+Lemma vad_preservation_spawn : forall m t1 t2 tid t,
+  valid_addresses m t1 ->
+  t1 --[e_spawn tid t]--> t2 ->
+  valid_addresses m t2.
+Proof.
+  intros. ind_tstep; inv_vad; eauto using valid_addresses.
+Qed.
+
+Lemma vad_preservation_spawned : forall m t1 t2 tid t,
+  valid_addresses m t1 ->
+  t1 --[e_spawn tid t]--> t2 ->
   valid_addresses m t.
 Proof.
-  intros. induction_tstep; inv_vad; eauto.
+  intros. ind_tstep; inv_vad; eauto.
 Qed.
 
 (* ------------------------------------------------------------------------- *)
@@ -209,10 +307,8 @@ Theorem vad_preservation : forall m1 m2 ths1 ths2 tid e,
   m1 / ths1 ~~[tid, e]~~> m2 / ths2 ->
   forall_program m2 ths2 (valid_addresses m2).
 Proof.
-  split_preservation.
-  - eauto using vad_preservation_spawn.
-  - eauto using vad_preservation_spawned.
-  - eauto using valid_addresses.
+  intros. split_preservation.
+  - eauto using vad_preservation_none.
   - eauto using vad_preservation_mem_alloc.
   - eauto using vad_preservation_alloc.
   - eauto using vad_preservation_unt_alloc.
@@ -220,7 +316,15 @@ Proof.
   - eauto using vad_preservation_mem_write.
   - eauto using vad_preservation_write.
   - eauto using vad_preservation_unt_write.
-  - eauto using vad_preservation_none.
+  - eauto using vad_preservation_mem_acq.
+  - eauto using vad_preservation_acq.
+  - eauto using vad_preservation_unt_acq.
+  - eauto using vad_preservation_mem_rel.
+  - eauto using vad_preservation_rel.
+  - eauto using vad_preservation_unt_rel.
+  - eauto using vad_preservation_spawn.
+  - eauto using vad_preservation_spawned.
+  - eauto using valid_addresses.
 Qed.
 
 (* ------------------------------------------------------------------------- *)
@@ -241,178 +345,290 @@ Qed.
 (* consistently-typed-references                                             *)
 (* ------------------------------------------------------------------------- *)
 
-Lemma ctr_mem_add : forall m t vT,
+Lemma ctr_subst : forall m t tx x,
+  consistently_typed_references m tx ->
+  consistently_typed_references m t ->
+  consistently_typed_references m <{[x := tx] t}>.
+Proof.
+  intros.
+  induction t; try inv_ctr; eauto using consistently_typed_references;
+  simpl; destruct str_eq_dec; eauto using consistently_typed_references.
+Qed.
+
+Lemma ctr_mem_add : forall m t tT,
   valid_addresses m t ->
   (* --- *)
   consistently_typed_references m t ->
-  consistently_typed_references (m +++ vT) t.
+  consistently_typed_references (m +++ tT) t.
 Proof.
   intros.
   induction t; eauto using consistently_typed_references;
   inv_vad; inv_ctr; eauto using consistently_typed_references;
-  (eapply ctr_refM || eapply ctr_refI); simpl_array; assumption.
+  (eapply ctr_refR || eapply ctr_refX || eapply ctr_refW);
+  simpl_array; assumption.
 Qed.
 
-Lemma ctr_mem_set : forall m t ad v T,
+Lemma ctr_mem_setX : forall m t te ad T,
   ad < #m ->
-  empty |-- v is T ->
-  m[ad].typ = <{{&T}}> ->
+  empty |-- te is T ->
+  m[ad].ty = `x&T` ->
   (* --- *)
   consistently_typed_references m t ->
-  consistently_typed_references m[ad <- (v, <{{&T}}>)] t.
+  consistently_typed_references m[ad <- (te, `x&T`)] t.
 Proof.
   intros.
   induction t; eauto using consistently_typed_references;
-  inv_ctr; eauto using consistently_typed_references;
-  (eapply ctr_refM || eapply ctr_refI);
-  match goal with H1 : _[?ad1].typ = _, H2 : _[?ad2].typ = _ |- _ =>
-    destruct (nat_eq_dec ad1 ad2); subst;
-    try (rewrite H1 in H2; inv H2)
+  invc_ctr; eauto using consistently_typed_references;
+  (eapply ctr_refR || eapply ctr_refX || eapply ctr_refW);
+  Array.sgs; trivial;
+  match goal with H1 : _[?ad1].ty = _, H2 : _[?ad2].ty = _ |- _ =>
+    rewrite H1 in H2; inv H2
   end;
-  simpl_array; trivial.
+  trivial.
 Qed.
 
-(* ------------------------------------------------------------------------- *)
+Lemma ctr_mem_setW : forall m t te ad T,
+  ad < #m ->
+  empty |-- te is T ->
+  m[ad].ty = `w&T` ->
+  (* --- *)
+  consistently_typed_references m t ->
+  consistently_typed_references m[ad <- (te, `w&T`)] t.
+Proof.
+  intros.
+  induction t; eauto using consistently_typed_references;
+  invc_ctr; eauto using consistently_typed_references;
+  (eapply ctr_refR || eapply ctr_refX || eapply ctr_refW);
+  Array.sgs; trivial;
+  match goal with H1 : _[?ad1].ty = _, H2 : _[?ad2].ty = _ |- _ =>
+    rewrite H1 in H2; inv H2
+  end;
+  trivial.
+Qed.
+
+Local Lemma ctr_ptm : forall m otid1 otid2 ad t T,
+  ad < #m ->
+  empty |-- t is T ->
+  m[ad].ty = `x&T` ->
+  (* --- *)
+  forall_memory m (consistently_typed_references m) ->
+  m[ad].tm = <{ptm otid1 t}> ->
+  consistently_typed_references m[ad <- (<{ptm otid2 t}>, `x&T`)] t.
+Proof.
+  intros * ? ? ? H Hptm.
+  specialize (H ad). simpl in H.
+  rewrite Hptm in H. invc_ctr.
+  eauto using type_of, ctr_mem_setX.
+Qed.
+
+(* none -------------------------------------------------------------------- *)
 
 Lemma ctr_preservation_none : forall m t1 t2,
   consistently_typed_references m t1 ->
-  t1 --[EF_None]--> t2 ->
+  t1 --[e_none]--> t2 ->
   consistently_typed_references m t2.
 Proof.
   intros.
-  induction_tstep; inv_ctr; eauto using consistently_typed_references.
-  inv_ctr. eauto using (must_subst consistently_typed_references).
+  ind_tstep; inv_ctr; eauto using consistently_typed_references.
+  inv_ctr. eauto using ctr_subst.
 Qed.
 
-(* ------------------------------------------------------------------------- *)
+(* alloc ------------------------------------------------------------------- *)
 
-Lemma ctr_preservation_mem_alloc : forall m t1 t2 v T,
+Lemma ctr_preservation_mem_alloc : forall m t1 t2 t T,
   well_typed_term t1 ->
   forall_memory m (valid_addresses m) ->
   valid_addresses m t1 ->
   consistently_typed_references m t1 ->
   (* --- *)
   forall_memory m (consistently_typed_references m) ->
-  t1 --[EF_Alloc (#m) v T]--> t2 ->
-  forall_memory (m +++ (v, T)) (consistently_typed_references (m +++ (v, T))).
+  t1 --[e_alloc (#m) t T]--> t2 ->
+  forall_memory (m +++ (t, T)) (consistently_typed_references (m +++ (t, T))).
 Proof.
   intros ** ad.
   decompose sum (lt_eq_lt_dec ad (#m)); subst; simpl_array;
   eauto using ctr_mem_add, consistently_typed_references; (* optimization *)
-  eauto using ctr_mem_add, (tstep_alloc_value consistently_typed_references).
+  eauto using ctr_mem_add, ctr_tstep_alloc_term.
 Qed.
 
-Lemma ctr_preservation_alloc : forall m t1 t2 v T,
+Lemma ctr_preservation_alloc : forall m t1 t2 t T,
   well_typed_term t1 ->
   valid_addresses m t1 ->
   (* --- *)
   consistently_typed_references m t1 ->
-  t1 --[EF_Alloc (#m) v T]--> t2 ->
-  consistently_typed_references (m +++ (v, T)) t2.
+  t1 --[e_alloc (#m) t T]--> t2 ->
+  consistently_typed_references (m +++ (t, T)) t2.
 Proof.
   intros * [T ?] **. generalize dependent T.
-  induction_tstep; intros; inv_ctr; inv_type; inv_vad;
+  ind_tstep; intros; inv_ctr; inv_typeof; inv_vad;
   eauto using ctr_mem_add, consistently_typed_references;
-  (eapply ctr_refM || eapply ctr_refI); simpl_array; trivial.
+  (eapply ctr_refR || eapply ctr_refX || eapply ctr_refW);
+  simpl_array; eauto using type_of, empty_eq_safe_empty.
 Qed.
 
-Lemma ctr_preservation_unt_alloc : forall m t1 t2 t ad v T,
-  valid_addresses m t ->
+Lemma ctr_preservation_unt_alloc : forall m t1 t2 tu ad t T,
+  valid_addresses m tu ->
   (* --- *)
-  consistently_typed_references m t ->
-  t1 --[EF_Alloc ad v T]--> t2 ->
-  consistently_typed_references (m +++ (v, T)) t.
+  consistently_typed_references m tu ->
+  t1 --[e_alloc ad t T]--> t2 ->
+  consistently_typed_references (m +++ (t, T)) tu.
 Proof.
   intros.
-  induction_tstep; eauto using ctr_mem_add, consistently_typed_references.
+  ind_tstep; eauto using ctr_mem_add, consistently_typed_references.
 Qed.
 
-(* ------------------------------------------------------------------------- *)
+(* read -------------------------------------------------------------------- *)
 
 Lemma ctr_preservation_read : forall m t1 t2 ad,
   consistently_typed_references m m[ad].tm ->
   (* --- *)
   consistently_typed_references m t1 ->
-  t1 --[EF_Read ad m[ad].tm]--> t2 ->
+  t1 --[e_read ad m[ad].tm]--> t2 ->
   consistently_typed_references m t2.
 Proof.
   intros.
-  induction_tstep; inv_ctr; eauto using consistently_typed_references.
+  ind_tstep; inv_ctr; eauto using consistently_typed_references.
 Qed.
 
-(* ------------------------------------------------------------------------- *)
+(* write ------------------------------------------------------------------- *)
 
-Lemma ctr_preservation_mem_write : forall m t1 t2 ad v T,
+Lemma ctr_preservation_mem_write : forall m t1 t2 ad t T,
   well_typed_term t1 ->
   consistently_typed_references m t1 ->
   (* --- *)
   ad < #m ->
   forall_memory m (consistently_typed_references m) ->
-  t1 --[EF_Write ad v T]--> t2 ->
-  forall_memory m[ad <- (v, T)] (consistently_typed_references m[ad <- (v, T)]).
+  t1 --[e_write ad t T]--> t2 ->
+  forall_memory m[ad <- (t, T)] (consistently_typed_references m[ad <- (t, T)]).
 Proof.
-  intros ** ad'.
-  assert (exists Tv, T = <{{&Tv}}>
-                  /\ empty |-- v is Tv
-                  /\ empty |-- m[ad].tm is Tv
-                  /\ m[ad].typ = <{{&Tv}}>)
-    as [? [? [? [? ?]]]] by eauto using consistently_typed_write_effect.
-  subst. Array.sgs;
-  eauto using ctr_mem_set, (tstep_write_value consistently_typed_references).
+  intros ** ?.
+  assert (Hctwe : exists Tm, T = `w&Tm`
+    /\ empty |-- t is Tm
+    /\ empty |-- m[ad].tm is Tm
+    /\ m[ad].ty = `w&Tm`)
+    by eauto using consistently_typed_write_effect.
+  decompose record Hctwe; subst.
+  Array.sgs; eauto using ctr_mem_setW, ctr_tstep_write_term.
 Qed.
 
-Lemma ctr_preservation_write : forall m t1 t2 ad v T,
+Lemma ctr_preservation_write : forall m t1 t2 ad t T,
   well_typed_term t1 ->
   (* --- *)
   ad < #m ->
   consistently_typed_references m t1 ->
-  t1 --[EF_Write ad v T]--> t2 ->
-  consistently_typed_references (m[ad <- (v, T)]) t2.
+  t1 --[e_write ad t T]--> t2 ->
+  consistently_typed_references (m[ad <- (t, T)]) t2.
 Proof.
   intros.
-  assert (exists Tv, T = <{{&Tv}}>
-                  /\ empty |-- v is Tv
-                  /\ empty |-- m[ad].tm is Tv
-                  /\ m[ad].typ = <{{&Tv}}>)
-    as [? [? [? [? ?]]]] by eauto using consistently_typed_write_effect.
-  induction_tstep; intros; inv_wtt; inv_ctr;
-  eauto using ctr_mem_set, consistently_typed_references.
+  assert (Hctwe : exists Tm, T = `w&Tm`
+    /\ empty |-- t is Tm
+    /\ empty |-- m[ad].tm is Tm
+    /\ m[ad].ty = `w&Tm`)
+    by eauto using consistently_typed_write_effect.
+  decompose record Hctwe; subst.
+  ind_tstep; intros; inv_wtt; inv_ctr;
+  eauto using ctr_mem_setW, consistently_typed_references.
 Qed.
 
-Lemma ctr_preservation_unt_write : forall m t1 t2 t ad v T,
+Lemma ctr_preservation_unt_write : forall m t1 t2 tu ad t T,
   well_typed_term t1 ->
   consistently_typed_references m t1 ->
   (* --- *)
   ad < #m ->
-  consistently_typed_references m t ->
-  t1 --[EF_Write ad v T]--> t2 ->
-  consistently_typed_references m[ad <- (v, T)] t.
+  consistently_typed_references m tu ->
+  t1 --[e_write ad t T]--> t2 ->
+  consistently_typed_references m[ad <- (t, T)] tu.
 Proof.
   intros.
-  assert (exists Tv, T = <{{&Tv}}>
-                  /\ empty |-- v is Tv
-                  /\ empty |-- m[ad].tm is Tv
-                  /\ m[ad].typ = <{{&Tv}}>)
-  as [? [? [? [? ?]]]] by eauto using consistently_typed_write_effect.
-  subst. eauto using ctr_mem_set.
+  assert (Hctwe : exists Tm, T = `w&Tm`
+    /\ empty |-- t is Tm
+    /\ empty |-- m[ad].tm is Tm
+    /\ m[ad].ty = `w&Tm`)
+    by eauto using consistently_typed_write_effect.
+  decompose record Hctwe; subst.
+  eauto using ctr_mem_setW.
 Qed.
 
-(* ------------------------------------------------------------------------- *)
+(* acq --------------------------------------------------------------------- *)
 
-Lemma ctr_preservation_spawn : forall m t1 t2 t,
+(* TODO *)
+
+(* rel --------------------------------------------------------------------- *)
+
+Lemma ctr_preservation_mem_rel : forall m1 m2 t1 t2 otid1 otid2 t tid ad T,
+  well_typed_term t1 ->
+  consistently_typed_references m1 t1 ->
+  (* --- *)
+  ad < #m1 ->
+  m1[ad].tm = <{ptm otid1 t}> ->
+  m2 = m1[ad <- (<{ptm otid2 t}>, `x&T`)] ->
+  (* --- *)
+  forall_memory m1 (consistently_typed_references m1) ->
+  t1 --[e_rel tid ad]--> t2 ->
+  forall_memory m2 (consistently_typed_references m2).
+Proof.
+  intros. subst.
+  assert (Hctwe : exists Tm, T = `w&Tm`
+    /\ empty |-- t is Tm
+    /\ empty |-- m[ad].tm is Tm
+    /\ m[ad].ty = `w&Tm`)
+    by eauto using consistently_typed_write_effect.
+  decompose record Hctwe; subst.
+
+
+  ind_tstep; invc_ctr; eauto. 
+  intros ?. Array.sgs.
+  - repeat clean. simpl.
+    eapply ctr_mem_setX; eauto.
+  - admit.
+  specialize (Hmvad ad'). simpl in *.
+  rewrite Hptm in Hmvad. invc Hmvad.
+  eauto using vad_mem_set, valid_addresses.
+Qed.
+
+Lemma vad_preservation_rel : forall m t1 t2 otid1 otid2 t tid ad T,
+  forall_memory m (valid_addresses m) ->
+  (* --- *)
+  ad < #m ->
+  m[ad].tm = <{ptm otid1 t}> ->
+  (* --- *)
+  valid_addresses m t1 ->
+  t1 --[e_rel tid ad]--> t2 ->
+  valid_addresses m[ad <- (<{ptm otid2 t}>, T)] t2.
+Proof.
+  intros.
+  ind_tstep; inv_vad; eauto using vad_mem_set, valid_addresses.
+Qed.
+
+Lemma vad_preservation_unt_rel : forall m t1 t2 tu otid1 otid2 t tid ad T,
+  forall_memory m (valid_addresses m) ->
+  (* --- *)
+  ad < #m ->
+  m[ad].tm = <{ptm otid1 t}> ->
+  (* --- *)
+  valid_addresses m tu ->
+  t1 --[e_rel tid ad]--> t2 ->
+  valid_addresses m[ad <- (<{ptm otid2 t}>, T)] tu.
+Proof.
+  eauto using vad_mem_set.
+Qed.
+
+(* spawn ------------------------------------------------------------------- *)
+
+Lemma ctr_preservation_spawn : forall m t1 t2 tid t,
   consistently_typed_references m t1 ->
-  t1 --[EF_Spawn t]--> t2 ->
+  t1 --[e_spawn tid t]--> t2 ->
   consistently_typed_references m t2.
 Proof.
-  intros. induction_tstep; inv_ctr; eauto using consistently_typed_references.
+  intros. ind_tstep; inv_ctr; eauto using consistently_typed_references.
 Qed.
 
-Lemma ctr_preservation_spawned : forall m t1 t2 t,
+Lemma ctr_preservation_spawned : forall m t1 t2 tid t,
   consistently_typed_references m t1 ->
-  t1 --[EF_Spawn t]--> t2 ->
+  t1 --[e_spawn tid t]--> t2 ->
   consistently_typed_references m t.
 Proof.
-  intros. induction_tstep; inv_ctr; eauto.
+  intros. ind_tstep; inv_ctr; eauto.
 Qed.
 
 (* ------------------------------------------------------------------------- *)
@@ -426,9 +642,7 @@ Theorem ctr_preservation : forall m1 m2 ths1 ths2 tid e,
   forall_program m2 ths2 (consistently_typed_references m2).
 Proof.
   split_preservation.
-  - eauto using ctr_preservation_spawn.
-  - eauto using ctr_preservation_spawned.
-  - eauto using consistently_typed_references.
+  - eauto using ctr_preservation_none.
   - eauto using ctr_preservation_mem_alloc.
   - eauto using ctr_preservation_alloc.
   - eauto using ctr_preservation_unt_alloc.
@@ -436,7 +650,15 @@ Proof.
   - eauto using ctr_preservation_mem_write.
   - eauto using ctr_preservation_write.
   - eauto using ctr_preservation_unt_write.
-  - eauto using ctr_preservation_none.
+  - admit.
+  - admit.
+  - admit.
+  - admit.
+  - admit.
+  - admit.
+  - eauto using ctr_preservation_spawn.
+  - eauto using ctr_preservation_spawned.
+  - eauto using consistently_typed_references.
 Qed.
 
 (* ------------------------------------------------------------------------- *)
@@ -486,9 +708,9 @@ Proof.
   - rewrite lookup_update_neq in IHHtype; eauto.
 Qed.
 
-Local Lemma nomut_safe_value : forall Gamma x t v T Tx,
-  value v ->
-  empty |-- v is Tx ->
+Local Lemma nomut_safe_value : forall Gamma x t tx T Tx,
+  value tx ->
+  empty |-- tx is Tx ->
   safe Gamma[x <== Tx] |-- t is T ->
   has_var x t ->
   no_mut v.
@@ -526,7 +748,7 @@ Qed.
 Lemma ss_preservation_mem_alloc : forall m t t' v T,
   forall_memory m safe_spawns ->
   safe_spawns t ->
-  t --[EF_Alloc (#m) v T]--> t' ->
+  t --[e_Alloc (#m) v T]--> t' ->
   forall_memory (m +++ (v, T)) safe_spawns.
 Proof.
   intros. unfold forall_memory.
@@ -536,7 +758,7 @@ Qed.
 Lemma ss_preservation_mem_write : forall m t t' ad v T,
   forall_memory m safe_spawns ->
   safe_spawns t ->
-  t --[EF_Write ad v T]--> t' ->
+  t --[e_Write ad v T]--> t' ->
   forall_memory m[ad <- (v, T)] safe_spawns.
 Proof.
   intros. unfold forall_memory.
@@ -545,7 +767,7 @@ Qed.
 
 Lemma ss_preservation_spawned : forall t1 t2 t,
   safe_spawns t1 ->
-  t1 --[EF_Spawn t]--> t2 ->
+  t1 --[e_Spawn t]--> t2 ->
   safe_spawns t.
 Proof.
   intros. induction_tstep; inv_ss; eauto using nomut_then_ss.
@@ -587,11 +809,11 @@ Qed.
 (* not-access                                                                *)
 (* ------------------------------------------------------------------------- *)
 
-Lemma nacc_mem_add : forall m t ad vT,
+Lemma nacc_mem_add : forall m t ad tT,
   ~ access (#m) m t ->
   (* --- *)
   ~ access ad m t ->
-  ~ access ad (m +++ vT) t.
+  ~ access ad (m +++ tT) t.
 Proof.
   intros ** Hacc.
   induction Hacc; do 2 inv_nacc; eauto.
@@ -633,7 +855,7 @@ Qed.
 
 Lemma nacc_preservation_none : forall m t1 t2 ad,
   ~ access ad m t1 ->
-  t1 --[EF_None]--> t2 ->
+  t1 --[e_None]--> t2 ->
   ~ access ad m t2.
 Proof.
   intros.
@@ -649,7 +871,7 @@ Lemma nacc_preservation_alloc : forall m t1 t2 ad v T,
   (* --- *)
   ad < #m ->
   ~ access ad m t1 ->
-  t1 --[EF_Alloc (#m) v T]--> t2 ->
+  t1 --[e_Alloc (#m) v T]--> t2 ->
   ~ access ad (m +++ (v, T)) t2.
 Proof.
   intros.
@@ -664,7 +886,7 @@ Lemma nacc_preservation_unt_alloc : forall m t1 t2 t ad ad' v T,
   valid_addresses m t ->
   (* --- *)
   ~ access ad m t ->
-  t1 --[EF_Alloc ad' v T]--> t2 ->
+  t1 --[e_Alloc ad' v T]--> t2 ->
   ~ access ad (m +++ (v, T)) t.
 Proof.
   eauto using nacc_mem_add, nacc_vad_length.
@@ -674,7 +896,7 @@ Qed.
 
 Lemma nacc_preservation_read : forall m t1 t2 ad ad',
   ~ access ad m t1 ->
-  t1 --[EF_Read ad' m[ad'].tm]--> t2 ->
+  t1 --[e_Read ad' m[ad'].tm]--> t2 ->
   ~ access ad m t2.
 Proof.
   intros. induction_tstep; inv_nacc; eauto with acc. inv_nacc. assumption.
@@ -684,7 +906,7 @@ Qed.
 
 Lemma nacc_preservation_write : forall m t1 t2 ad ad' v T,
   ~ access ad m t1 ->
-  t1 --[EF_Write ad' v T]--> t2 ->
+  t1 --[e_Write ad' v T]--> t2 ->
   ~ access ad (m[ad' <- (v, T)]) t2.
 Proof.
   intros.
@@ -697,7 +919,7 @@ Lemma nacc_preservation_unt_write : forall m t1 t2 t ad ad' v T,
   (access ad' m t -> ~ unsafe_access ad' m t1) ->
   (* --- *)
   ~ access ad m t ->
-  t1 --[EF_Write ad' v T]--> t2 ->
+  t1 --[e_Write ad' v T]--> t2 ->
   ~ access ad m[ad' <- (v, T)] t.
 Proof.
   intros * ? Hsms **.
@@ -710,7 +932,7 @@ Qed.
 
 Lemma nacc_preservation_spawn : forall m t1 t2 t ad,
   ~ access ad m t1 ->
-  t1 --[EF_Spawn t]--> t2 ->
+  t1 --[e_Spawn t]--> t2 ->
   ~ access ad m t2.
 Proof.
   intros ** ?. induction_tstep; try inv_nacc; inv_acc; eauto.
@@ -744,11 +966,11 @@ Qed.
 (* not-unsafe-access                                                         *)
 (* ------------------------------------------------------------------------- *)
 
-Lemma nuacc_mem_add : forall m t ad vT,
+Lemma nuacc_mem_add : forall m t ad tT,
   ~ unsafe_access (#m) m t ->
   (* --- *)
   ~ unsafe_access ad m t ->
-  ~ unsafe_access ad (m +++ vT) t.
+  ~ unsafe_access ad (m +++ tT) t.
 Proof.
   intros ** Huacc.
   induction Huacc; inv_nuacc; eauto using unsafe_access.
@@ -775,11 +997,11 @@ Proof.
   Array.sgs; eauto using unsafe_access.
 Qed.
 
-Lemma nuacc_mem_set2 : forall m t ad ad' vT,
+Lemma nuacc_mem_set2 : forall m t ad ad' tT,
   ~ unsafe_access ad' m t ->
   (* --- *)
   ~ unsafe_access ad m t ->
-  ~ unsafe_access ad m[ad' <- vT] t.
+  ~ unsafe_access ad m[ad' <- tT] t.
 Proof.
   intros ** Huacc.
   induction Huacc; inv_nuacc; inv_nuacc; eauto.
@@ -791,7 +1013,7 @@ Qed.
 
 Lemma nuacc_preservation_none : forall m t1 t2 ad,
   ~ unsafe_access ad m t1 ->
-  t1 --[EF_None]--> t2 ->
+  t1 --[e_None]--> t2 ->
   ~ unsafe_access ad m t2.
 Proof.
   intros ** Huacc.
@@ -807,7 +1029,7 @@ Lemma nuacc_preservation_alloc : forall m t1 t2 ad v T,
   (* --- *)
   ad < #m ->
   ~ unsafe_access ad m t1 ->
-  t1 --[EF_Alloc (#m) v T]--> t2 ->
+  t1 --[e_Alloc (#m) v T]--> t2 ->
   ~ unsafe_access ad (m +++ (v, T)) t2.
 Proof.
   intros ** ?.
@@ -821,7 +1043,7 @@ Lemma nuacc_preservation_unt_alloc : forall m t1 t2 t ad ad' v T,
   valid_addresses m t ->
   (* --- *)
   ~ unsafe_access ad m t ->
-  t1 --[EF_Alloc ad' v T]--> t2 ->
+  t1 --[e_Alloc ad' v T]--> t2 ->
   ~ unsafe_access ad (m +++ (v, T)) t.
 Proof.
   eauto using nuacc_mem_add, nuacc_vad_length.
@@ -835,7 +1057,7 @@ Lemma nuacc_preservation_read : forall m t1 t2 ad ad',
   consistently_typed_references m t1 ->
   (* --- *)
   ~ unsafe_access ad m t1 ->
-  t1 --[EF_Read ad' m[ad'].tm]--> t2 ->
+  t1 --[e_Read ad' m[ad'].tm]--> t2 ->
   ~ unsafe_access ad m t2.
 Proof.
   intros ** ?.
@@ -851,12 +1073,12 @@ Qed.
 
 Lemma nuacc_preservation_write : forall m t1 t2 ad ad' v T,
   ~ unsafe_access ad m t1 ->
-  t1 --[EF_Write ad' v T]--> t2 ->
+  t1 --[e_Write ad' v T]--> t2 ->
   ~ unsafe_access ad m[ad' <- (v, T)] t2.
 Proof.
   assert (forall m t t' ad ad' v T,
     ~ unsafe_access ad m t ->
-    t --[EF_Write ad' v T]--> t' ->
+    t --[e_Write ad' v T]--> t' ->
     ~ unsafe_access ad m v)
     by (intros; induction_tstep; eauto using unsafe_access).
   (* main proof *)
@@ -870,7 +1092,7 @@ Lemma nuacc_preservation_unt_write : forall m t1 t2 t ad ad' v T,
   (access ad' m t -> ~ unsafe_access ad' m t1) ->
   (* --- *)
   ~ unsafe_access ad m t ->
-  t1 --[EF_Write ad' v T]--> t2 ->
+  t1 --[e_Write ad' v T]--> t2 ->
   ~ unsafe_access ad m[ad' <- (v, T)] t.
 Proof.
   intros * ? Hsms **.
@@ -883,7 +1105,7 @@ Qed.
 
 Lemma nuacc_preservation_spawn : forall m t1 t2 t ad,
   ~ unsafe_access ad m t1 ->
-  t1 --[EF_Spawn t]--> t2 ->
+  t1 --[e_Spawn t]--> t2 ->
   ~ unsafe_access ad m t2.
 Proof.
   intros ** ?. induction_tstep; inv_uacc; eauto; inv_nuacc; eauto.
@@ -952,12 +1174,12 @@ Local Lemma step_write_sms_helper : forall m t ad v ths tid tid' T,
   tid <> tid' ->
   forall_threads ths well_typed_term ->
   safe_memory_sharing m ths ->
-  ths[tid] --[EF_Write ad v T]--> t ->
+  ths[tid] --[e_Write ad v T]--> t ->
   ~ access ad m ths[tid'].
 Proof.
   assert (forall m t t' ad v T Te,
     empty |-- t is T ->
-    t --[EF_Write ad v Te]--> t' ->
+    t --[e_Write ad v Te]--> t' ->
     unsafe_access ad m t
   ). {
     intros. generalize dependent T.
@@ -984,7 +1206,7 @@ Local Ltac destruct_sms ths tid tid1 tid2 :=
 
 Local Lemma sms_tstep_none_preservation : forall m t ths tid,
   safe_memory_sharing m ths ->
-  ths[tid] --[EF_None]--> t ->
+  ths[tid] --[e_None]--> t ->
   safe_memory_sharing m ths[tid <- t].
 Proof.
   intros ** tid1 tid2 **. destruct_sms ths tid tid1 tid2; simpl_array;
@@ -996,7 +1218,7 @@ Local Lemma sms_tstep_alloc_preservation : forall m t v ths tid T,
   forall_threads ths (valid_addresses m) ->
   (* --- *)
   safe_memory_sharing m ths ->
-  ths[tid] --[EF_Alloc (#m) v T]--> t ->
+  ths[tid] --[e_Alloc (#m) v T]--> t ->
   safe_memory_sharing (m +++ (v, T)) ths[tid <- t].
 Proof.
   intros * ? Hvad ** tid1 tid2 ** Huacc.
@@ -1017,7 +1239,7 @@ Local Lemma sms_tstep_read_preservation : forall m t ad ths tid,
   forall_threads ths (consistently_typed_references m) ->
   (* --- *)
   safe_memory_sharing m ths ->
-  ths[tid] --[EF_Read ad m[ad].tm]--> t ->
+  ths[tid] --[e_Read ad m[ad].tm]--> t ->
   safe_memory_sharing m ths[tid <- t].
 Proof.
   intros * ? Hwtt ** tid1 tid2 **. destruct (Hwtt tid1).
@@ -1029,7 +1251,7 @@ Local Lemma sms_tstep_write_preservation : forall m ths t tid ad v T,
   forall_threads ths well_typed_term ->
   (* --- *)
   safe_memory_sharing m ths ->
-  ths[tid] --[EF_Write ad v T]--> t ->
+  ths[tid] --[e_Write ad v T]--> t ->
   safe_memory_sharing m[ad <- (v, T)] ths[tid <- t].
 Proof.
   intros ** tid1 tid2 ** Huacc.
@@ -1054,7 +1276,7 @@ Local Lemma sms_tstep_spawn_preservation : forall m ths t block tid,
   (* --- *)
   tid < #ths ->
   safe_memory_sharing m ths ->
-  ths[tid] --[EF_Spawn block]--> t ->
+  ths[tid] --[e_Spawn block]--> t ->
   safe_memory_sharing m (ths[tid <- t] +++ block).
 Proof.
   intros ** tid1 tid2 **.
