SemExt.v
@@ -1,0 +1,189 @@
+From Coq Require Import Lia.
+
+From Elo Require Import Util.
+From Elo Require Import Array.
+From Elo Require Import Map.
+From Elo Require Import Sem.
+
+(* ------------------------------------------------------------------------- *)
+(* typeof inversion & induction                                              *)
+(* ------------------------------------------------------------------------- *)
+
+Ltac _typeof tt :=
+  match goal with
+  | H : _ |-- <{unit     }> is _ |- _ => tt H
+  | H : _ |-- <{nat _    }> is _ |- _ => tt H
+  | H : _ |-- <{var _    }> is _ |- _ => tt H
+  | H : _ |-- <{fn _ _ _ }> is _ |- _ => tt H
+  | H : _ |-- <{call _ _ }> is _ |- _ => tt H
+  | H : _ |-- <{& _ : _  }> is _ |- _ => tt H
+  | H : _ |-- <{new _ : _}> is _ |- _ => tt H
+  | H : _ |-- <{* _      }> is _ |- _ => tt H
+  | H : _ |-- <{_ := _   }> is _ |- _ => tt H
+  | H : _ |-- <{acq _ _  }> is _ |- _ => tt H
+  | H : _ |-- <{cr _ _   }> is _ |- _ => tt H
+  | H : _ |-- <{ptm _ _  }> is _ |- _ => tt H
+  | H : _ |-- <{spawn _  }> is _ |- _ => tt H
+  end.
+
+Ltac inv_typeof  := _typeof inv.
+Ltac invc_typeof := _typeof invc.
+
+Ltac ind_typeof := match goal with H : _ |-- _ is _ |- _ => induction H end.
+
+(* ------------------------------------------------------------------------- *)
+(* step inversion & induction                                                *)
+(* ------------------------------------------------------------------------- *)
+
+Ltac _tstep tt := match goal with H : _     --[_]-->    _     |- _ => tt H end.
+Ltac _mstep tt := match goal with H : _ / _ ==[_]==>    _ / _ |- _ => tt H end.
+Ltac _cstep tt := match goal with H : _ / _ ~~[_, _]~~> _ / _ |- _ => tt H end.
+Ltac _ustep tt := match goal with H : _ / _ ~~[_]~~>*   _ / _ |- _ => tt H end.
+
+Ltac inv_tstep := _tstep inv.
+Ltac inv_mstep := _mstep inv.
+Ltac inv_cstep := _cstep inv.
+Ltac inv_ustep := _ustep inv.
+
+Ltac invc_tstep := _tstep invc.
+Ltac invc_mstep := _mstep invc.
+Ltac invc_cstep := _cstep invc.
+Ltac invc_ustep := _ustep invc.
+
+Ltac ind_tstep :=
+  match goal with H : _ --[?e]--> _ |- _ =>
+    remember e eqn:Heq; induction H; inv Heq
+  end.
+
+Ltac ind_ustep :=
+  match goal with H : _ / _ ~~[_]~~>* _ / _ |- _ =>
+    induction H as [| ? ? ? ? ? ? ? ? ? Hustep ? Hcstep]
+  end.
+
+(* ------------------------------------------------------------------------- *)
+(* decidability & equality                                                   *)
+(* ------------------------------------------------------------------------- *)
+
+Lemma value_dec : forall t,
+  value t \/ ~ value t.
+Proof.
+  intros. induction t; eauto using value; right; intros F; inv F.
+Qed.
+
+Lemma styp_eq_dec : forall (T1 T2 : sty), {T1 = T2} + {T1 <> T2}
+with  typ_eq_dec  : forall (T1 T2 : ty),  {T1 = T2} + {T1 <> T2}.
+Proof.
+  - decide equality.
+  - decide equality.
+Qed.
+
+Lemma tm_eq_dec : forall (t1 t2 : tm),
+  {t1 = t2} + {t1 <> t2}.
+Proof.
+  intros.
+  decide equality; eauto using nat_eq_dec, str_eq_dec, typ_eq_dec.
+  decide equality. eauto using nat_eq_dec.
+Qed.
+
+Lemma eff_eq_dec : forall (e1 e2 : eff),
+  {e1 = e2} + {e1 <> e2}.
+Proof.
+  intros. decide equality; eauto using nat_eq_dec, typ_eq_dec, tm_eq_dec.
+Qed.
+
+(* ------------------------------------------------------------------------- *)
+(* forall properties                                                         *)
+(* ------------------------------------------------------------------------- *)
+
+Definition forall_memory (m : mem) (P : tm -> _) : Prop :=
+  forall_array mem_default (fun tT => P (fst tT)) m.
+
+Definition forall_threads (ths : threads) (P : tm -> _) : Prop :=
+  forall_array tm_default P ths.
+
+Definition forall_program (m : mem) (ths : threads) (P : tm -> _) : Prop :=
+  (forall_memory m P) /\ (forall_threads ths P).
+
+#[export] Hint Unfold forall_program : core.
+
+(* ------------------------------------------------------------------------- *)
+(* determinism                                                               *)
+(* ------------------------------------------------------------------------- *)
+
+Lemma deterministic_typing : forall Gamma t T1 T2,
+  Gamma |-- t is T1 ->
+  Gamma |-- t is T2 ->
+  T1 = T2.
+Proof.
+  intros * Htype1. generalize dependent T2.
+  induction Htype1; intros ? Htype2; inv Htype2; eauto;
+  repeat match goal with
+  | IH : forall _, _ |-- ?t is _ -> _, H : _ |-- ?t is _ |- _ =>
+    eapply IH in H; subst
+  end;
+  congruence.
+Qed.
+
+Ltac apply_deterministic_typing :=
+  match goal with
+  | H1 : _ |-- ?t is ?T1
+  , H2 : _ |-- ?t is ?T2
+  |- _ =>
+    assert (Heq : T1 = T2) by eauto using deterministic_typing; subst;
+    try (invc Heq)
+  end.
+
+(* ------------------------------------------------------------------------- *)
+(* auxiliary lemmas                                                          *)
+(* ------------------------------------------------------------------------- *)
+
+Lemma tstep_tid_bound : forall t ths tid e,
+  ths[tid] --[e]--> t ->
+  tid < #ths.
+Proof.
+  intros. decompose sum (lt_eq_lt_dec tid (#ths)); subst; trivial; simpl_array;
+  solve [lia | inv_tstep].
+Qed.
+
+Lemma mstep_tid_bound : forall m m' t' ths tid e,
+  m / ths[tid] ==[e]==> m' / t' ->
+  tid < #ths.
+Proof.
+  intros. inv_mstep; eauto using tstep_tid_bound.
+Qed.
+
+Lemma cstep_tid_bound : forall m m' ths ths' tid e,
+  m / ths ~~[tid, e]~~> m' / ths' ->
+  tid < #ths.
+Proof.
+  intros. inv_cstep; trivial.
+Qed.
+
+(* ------------------------------------------------------------------------- *)
+(* context equivalence                                                       *)
+(* ------------------------------------------------------------------------- *)
+
+Lemma ctx_eqv_safe : forall Gamma1 Gamma2,
+  Gamma1 === Gamma2 ->
+  safe Gamma1 === safe Gamma2.
+Proof.
+  unfold map_eqv, safe. intros * Heq k.
+  specialize (Heq k). rewrite Heq. trivial.
+Qed.
+
+Lemma ctx_eqv_typeof : forall Gamma1 Gamma2 t T,
+  Gamma1 === Gamma2 ->
+  Gamma1 |-- t is T ->
+  Gamma2 |-- t is T.
+Proof.
+  intros. generalize dependent Gamma2. ind_typeof; intros;
+  eauto using MapEqv.lookup, MapEqv.update_eqv, type_of, ctx_eqv_safe.
+Qed.
+
+Lemma ctx_eqv_safe_lookup : forall Gamma x,
+  Gamma x = None ->
+  (safe Gamma) x = None.
+Proof.
+  unfold safe. intros * H. rewrite H. reflexivity.
+Qed.
+
