Temp.v
@@ -1,0 +1,49 @@
+From Elo Require Import Core.
+From Elo Require Import Properties.
+
+Lemma nwacc_alloc : forall m t t' ad te T,
+  ad < #m ->
+  ~ write_access ad m t ->
+  t --[e_alloc (#m) te T]--> t' ->
+  ~ write_access ad m t'.
+Proof.
+  intros. ind_tstep.
+  - inv_nwacc. eauto with wacc.
+  - inv_nwacc. eauto with wacc.
+  - inv_nwacc. eauto with wacc.
+  - inv_nwacc. eauto with wacc.
+  - inv_nwacc. eauto with wacc.
+  - inv_nwacc.
+    intros ?.
+    eapply H0. clear H0.
+    invc H2.
+    + Array.simpl_array. simpl in *. inv H5.
+    +
+  - inv_nwacc. eauto with wacc.
+  - inv_nwacc. eauto with wacc.
+  - inv_nwacc. eauto with wacc.
+  - inv_nwacc. eauto with wacc.
+  - inv_nwacc. eauto with wacc.
+  - inv_nwacc. eauto with wacc.
+Abort.
+
+Lemma nwacc_spawn : forall m t t' te ad,
+  ~ write_access ad m t ->
+  t --[e_spawn te]--> t' ->
+  ~ write_access ad m t'.
+Proof.
+  intros. ind_tstep; try inv_nwacc; eauto with wacc.
+Qed.
+
+Lemma todo : forall m m' ths ths' ad tid e,
+  ~ write_access ad m ths[tid] ->
+  m / ths ~~[tid, e]~~> m' / ths' ->
+  write_access ad m ths'[tid] ->
+  exists ad' t, e = e_acq ad' t.
+Proof.
+  intros * Hnwacc ? Hwacc.
+  invc_cstep; Array.simpl_array.
+  - contradict Hwacc. eauto using nwacc_spawn.
+  - invc_mstep. 
+    +
+Qed.
